thys/CAVA_Automata/CAVA_Base/Code_String.thy
@@ -6,41 +6,6 @@ theory Code_String
 imports
   (*"HOL-Library.List_lexord"*)
   Collections.Refine_Dflt      
-  "HOL-Library.Code_Char"
 begin
 
-(* TODO: Move to Collections *)
-instantiation String.literal :: hashable
-begin
-  definition hashcode_literal :: "String.literal \<Rightarrow> uint32" 
-    where "hashcode_literal s = hashcode (String.explode s)"
-
-  definition def_hashmap_size_literal 
-    :: "String.literal itself \<Rightarrow> nat" where
-    "def_hashmap_size_literal _ = 10"
-
-  instance proof
-  qed (simp_all only: def_hashmap_size_literal_def)
-end
-
-(* Append on literal strings -- allows for easier written exceptions *)
-
-context 
-  includes literal.lifting
-begin
-
-lift_definition literal_append 
-  :: "String.literal \<Rightarrow> String.literal \<Rightarrow> String.literal"  (infixr "@@" 65)
-  is "(@)" .
-
-end
-
-lifting_update literal.lifting
-lifting_forget literal.lifting
-
-code_printing
-  constant literal_append \<rightharpoonup>
-    (SML) infixr 5 "^"
-    and (Haskell) infixr 5 "++"
-    and (OCaml) infixr 5 "^"
 end
