thys/JinjaThreads/Basic/Basic_Main.thy
@@ -2,7 +2,6 @@ theory Basic_Main
 imports Main
   "HOL-Library.Sublist"
   "HOL-Library.Transitive_Closure_Table"
-  "HOL-Library.Code_Char"
   "HOL-Library.Predicate_Compile_Alternative_Defs"
   "HOL-Library.Dlist"
   Set_without_equal
