thys/Paraconsistency/Paraconsistency.thy
@@ -183,8 +183,8 @@ where
 
 fun string_of_nat :: "nat \<Rightarrow> string"
 where
-  "string_of_nat n = (if n < 10 then [char_of_nat (48 + n)] else
-      string_of_nat (n div 10) @ [char_of_nat (48 + (n mod 10))])"
+  "string_of_nat n = (if n < 10 then [char_of (48 + n)] else
+      string_of_nat (n div 10) @ [char_of (48 + (n mod 10))])"
 
 fun string_tv :: "tv \<Rightarrow> string"
 where
